failing at proving things

sva_soundness.v
@@ -1,8 +1,24 @@
+(** SVA soundness proofs *)
+
+(* CompCert Imports *)
 Add LoadPath "./CompCert-Toolkit".
+Require Import Maps.
+Require Import Integers.
+Require Import AST.
+Require Import Smallstep.
+Require Import Globalenvs.
+Require Import Events.
+
+(* SF imports *)
+Require Import SfLib.
+
+(* SVA imports *)
 Require Import sva_typing.
 Require Import sva_dynamic.
-Require Import SfLib.
-Require Import Maps.
+Require Import sva_allocator.
+
+(* Coq standard library imports *)
+Require Import ListSet.
 
 Tactic Notation "exp_cases" tactic(first) ident(c) :=
   first;
@@ -27,15 +43,93 @@ Proof.
   Case "SS8". apply H.
 Qed.
 
-Inductive crazyshit : tipe -> Prop :=
-  | Int_wf : crazyshit Int_t
-  | Pts_wf : crazyshit Int_t
-  | Handle_wf : crazyshit Int_t
-  | Unknown_wf : crazyshit Int_t.
+Inductive crazyshit : tipe -> VarEnv -> LiveRegions -> sva_heap -> value -> Prop :=
+  | Int_wf : forall n venv l h,
+      crazyshit Int_t venv l h (Int n)
+  | Pts_wf : forall venv l tau rho h,
+      crazyshit (Pts_t tau rho) venv l h Uninit
+  | Pts_wf2 : forall venv l tau rho b ri h,
+      PTree.get rho l = Some ri ->
+      set_In b (RS ri) -> 
+      crazyshit (Pts_t tau rho) venv l h (Pointer b Int.zero)
+  | Handle_wf : forall venv l tau rho h,
+      crazyshit (Handle_t rho tau) venv l h (Region rho)
+  | Unknown_wf : forall venv l b h,
+      crazyshit Unknown_t venv l h (Byte b).
 
-Inductive wf_env : context -> VarEnv -> LiveRegions -> Prop :=
-  | blah : forall Gamma Delta venv l x rho foo foo' bar bar',
-      iff (PTree.get x Gamma = Some foo) (PTree.get x venv = Some foo') ->
-      iff (PTree.get rho Delta = Some bar) (PTree.get rho l = Some bar') ->
-      (PTree.get x venv = Some foo) -> 
-      wf_env (Gamma, Delta) venv l.
+(* Skipping invariant 5 and 6 ... *)
+Inductive wf_env : context -> VarEnv -> LiveRegions -> sva_heap -> Prop :=
+  | blah : forall Gamma Delta venv l h,
+      ( forall x tau v,
+        iff (PTree.get x Gamma = Some tau) (PTree.get x venv = Some v) ) ->
+      ( forall rho tau region,
+        iff (PTree.get rho Delta = Some tau) (PTree.get rho l = Some region) ) ->
+      ( forall x tau v,
+        PTree.get x venv = Some v -> 
+        has_type_exp (Gamma,Delta) (Var x) tau ->
+        crazyshit tau venv l h v ) ->
+      ( forall rho tau b ri,
+        PTree.get rho l = Some ri ->
+        PTree.get rho Delta = Some tau ->
+        set_In b (RS ri) ->
+        crazyshit tau venv l h (Pointer b Int.zero) ) ->
+      ( forall rho ri b,
+        PTree.get rho l = Some ri ->
+        In b (F ri) ->
+        set_In b (RS ri) ) ->
+      ( forall rho1 rho2 b1 b2 ri1 ri2,
+        rho1 <> rho2 ->
+        PTree.get rho1 l = Some ri1 ->
+        PTree.get rho2 l = Some ri2 ->
+        set_In b1 (RS ri1) -> not (set_In b1 (RS ri2)) /\
+        set_In b2 (RS ri2) -> not (set_In b2 (RS ri1)) ) ->
+      wf_env (Gamma, Delta) venv l h.
+
+(*
+Lemma UpdateLemma1 : forall Gamma Delta venv l h rho tau b o v ri,
+  wf_env (Gamma,Delta) venv l h ->
+  PTree.get rho Delta = Some tau ->
+  PTree.get rho l = Some ri ->
+  set_In b (RS ri) ->
+  crazyshit tau venv l h v ->
+  wf_env (Gamma,Delta) venv l (sva_store h b o Mint32 v).
+Proof.
+  intros. unfold sva_store.
+  destruct (Memory.Mem.store Mint32 (sva_mem h) b (Int.unsigned o) (val2CCval v)).
+  inversion H. *)
+
+Definition ge0 := Genv.empty_genv nat nat.
+
+Lemma trace_E0 : forall t1 t2,
+  E0 = t1 ** t2 ->
+  t1 = E0 /\ t2 = E0.
+Proof.
+  destruct t1; intros; unfold E0; try solve [ auto | discriminate]. 
+Qed.
+
+Lemma TrivWTF : forall venv l e h venv' l' e' h',
+  l = l' -> e = e' -> h = h' -> venv = venv' ->
+  (state_e venv l e h) = (state_e venv' l' e' h').
+  intros. subst. reflexivity.
+Qed.
+
+Lemma TrivWTF2 : forall venv l e h venv' l' e' h',
+  (state_e venv l e h) = (state_e venv' l' e' h') ->
+  (l = l' /\ e = e' /\ h = h' /\ venv = venv').
+  intros. split. inversion H. reflexivity.
+  split. inversion H. reflexivity.
+  split. inversion H. reflexivity.
+  inversion H. reflexivity.
+Qed.
+
+Check star_ind.
+Check step_exp.
+Lemma R2star : forall s venv l e h s' venv' l' e' h' x,
+  s = state_e venv l e h ->
+  s' = state_e venv' l' e' h' ->
+  star step_exp tt s E0 s' ->
+  star step_stmt tt (state_s venv l (Assign x e) h) E0 (state_s venv' l' (Assign x e') h').
+Proof.
+  intros. induction H1. subst. inversion H0. subst. constructor. 
+  subst. 
+Qed.
